Allow user supplied modified registers for inline assembly

vale/code/arch/x64/interop/Vale.AsLowStar.ValeSig.fst
@@ -39,31 +39,16 @@ let vale_save_reg (r:MS.reg) (s0 s1:V.va_state) =
 let vale_save_xmm (r:MS.xmm) (s0 s1:V.va_state) =
   VS.eval_xmm r s0 == VS.eval_xmm r s1
 
-let vale_calling_conventions (s0 s1:V.va_state) =
+let vale_calling_conventions 
+  (s0 s1:V.va_state) 
+  (regs_modified:MS.reg -> bool)
+  (xmms_modified:MS.xmm -> bool) =
   let open MS in
-  vale_save_reg Rbx s0 s1 /\
-  (IA.win ==> vale_save_reg Rsi s0 s1) /\
-  (IA.win ==> vale_save_reg Rdi s0 s1) /\
-  vale_save_reg Rbp s0 s1 /\
-  (IA.win ==> vale_save_reg Rsp s0 s1) /\ // TODO: also needed for !IA.win
-  vale_save_reg R12 s0 s1 /\
-  vale_save_reg R13 s0 s1 /\
-  vale_save_reg R14 s0 s1 /\
-  vale_save_reg R15 s0 s1 /\
-  (IA.win ==>
-    vale_save_xmm 6 s0 s1 /\
-    vale_save_xmm 7 s0 s1 /\
-    vale_save_xmm 8 s0 s1 /\
-    vale_save_xmm 9 s0 s1 /\
-    vale_save_xmm 10 s0 s1 /\
-    vale_save_xmm 11 s0 s1 /\
-    vale_save_xmm 12 s0 s1 /\
-    vale_save_xmm 13 s0 s1 /\
-    vale_save_xmm 14 s0 s1 /\
-    vale_save_xmm 15 s0 s1
-  ) /\
-  s1.VS.ok
-
+  s1.VS.ok /\
+  (forall (r:MS.reg).
+    not (regs_modified r) ==> vale_save_reg r s0 s1) /\
+  (forall (x:MS.xmm).
+    not (xmms_modified x) ==> vale_save_xmm x s0 s1)
 
 [@__reduce__]
 let modified_arg_mloc (x:arg) : GTot ME.loc =
@@ -125,6 +110,8 @@ let disjoint_or_eq (l:list arg) =
 
 [@__reduce__] unfold
 let vale_sig_nil #n
+                 (regs_modified:MS.reg -> bool)
+                 (xmms_modified:MS.xmm -> bool)
                  (args:list arg)
                  (code:V.va_code)
                  (pre:vale_pre_tl n [])
@@ -138,13 +125,15 @@ let vale_sig_nil #n
        let va_s1 = state_of r in
        let f = fuel_of r in
        V.eval_code code va_s0 f va_s1 /\
-       vale_calling_conventions va_s0 va_s1 /\
+       vale_calling_conventions va_s0 va_s1 regs_modified xmms_modified /\
        elim_nil post va_s0 stack_b va_s1 f /\
        readable args VS.(va_s1.mem) /\
        ME.modifies (mloc_modified_args (arg_of_sb stack_b :: args)) va_s0.VS.mem va_s1.VS.mem))
 
 [@__reduce__]
 let rec vale_sig_tl #n
+                    (regs_modified:MS.reg -> bool)
+                    (xmms_modified:MS.xmm -> bool)
                     (#dom:list td)
                     (args:list arg)
                     (code:V.va_code)
@@ -153,43 +142,58 @@ let rec vale_sig_tl #n
   : Type =
     match dom with
     | [] ->
-      vale_sig_nil args code pre post
+      vale_sig_nil regs_modified xmms_modified args code pre post
 
     | hd::tl ->
       x:td_as_type hd ->
-      vale_sig_tl #n #tl ((|hd,x|)::args) code (elim_1 pre x) (elim_1 post x)
+      vale_sig_tl #n regs_modified xmms_modified #tl ((|hd,x|)::args) code (elim_1 pre x) (elim_1 post x)
 
 
 [@__reduce__]
 let elim_vale_sig_nil #n #code
+                       (#regs_modified:MS.reg -> bool)
+                       (#xmms_modified:MS.xmm -> bool)
                        (#args:list arg)
                        (#pre:vale_pre_tl n [])
                        (#post:vale_post_tl n [])
-                       (v:vale_sig_tl #n #[] args code pre post)
-    : vale_sig_nil args code pre post
+                       (v:vale_sig_tl #n regs_modified xmms_modified #[] args code pre post)
+    : vale_sig_nil regs_modified xmms_modified args code pre post
     = v
 
 [@__reduce__]
 let elim_vale_sig_cons #n #code
+                       (#regs_modified:MS.reg -> bool)
+                       (#xmms_modified:MS.xmm -> bool)
                        (hd:td)
                        (tl:list td)
                        (args:list arg)
                        (pre:vale_pre_tl n (hd::tl))
                        (post:vale_post_tl n (hd::tl))
-                       (v:vale_sig_tl args code pre post)
+                       (v:vale_sig_tl regs_modified xmms_modified args code pre post)
     : x:td_as_type hd
-    -> vale_sig_tl ((|hd, x|)::args) code (elim_1 pre x) (elim_1 post x)
+    -> vale_sig_tl regs_modified xmms_modified ((|hd, x|)::args) code (elim_1 pre x) (elim_1 post x)
     = v
 
 [@__reduce__]
 let vale_sig #n (#dom:list td)
+             (regs_modified:MS.reg -> bool)
+             (xmms_modified:MS.xmm -> bool)
              (pre:vale_pre n dom)
              (post:vale_post n dom)
   : Type =
     code:V.va_code ->
     win:bool ->
     vale_sig_tl
+      regs_modified
+      xmms_modified
       []
       code
       (pre code)
       (post code)
+
+[@__reduce__]
+let vale_sig_stdcall #n #dom = vale_sig #n #dom IX64.regs_modified_stdcall IX64.xmms_modified_stdcall
+
+[@__reduce__]
+let vale_calling_conventions_stdcall (s0 s1:VS.state) = 
+  vale_calling_conventions s0 s1 IX64.regs_modified_stdcall IX64.xmms_modified_stdcall
