vale/code/arch/x64/interop/Vale.AsLowStar.Test.fst
@@ -35,12 +35,12 @@ let dom : IX64.arity_ok_stdcall td =
 assume val n : IX64.max_slots
 assume val pre : VSig.vale_pre n dom
 assume val post : VSig.vale_post n dom
-assume val v: VSig.vale_sig pre post
+assume val v: VSig.vale_sig_stdcall pre post
 assume val c: V.va_code
 
 [@__reduce__]
-let call_c_t = IX64.as_lowstar_sig_t_weak IX64.max_stdcall IX64.arg_reg_stdcall Interop.down_mem c n dom [] _ _ (W.mk_prediction c dom [] (v c IA.win))
-let call_c : call_c_t = IX64.wrap_weak IX64.max_stdcall IX64.arg_reg_stdcall Interop.down_mem c n dom (W.mk_prediction c dom [] (v c IA.win))
+let call_c_t = IX64.as_lowstar_sig_t_weak IX64.max_stdcall IX64.arg_reg_stdcall IX64.regs_modified_stdcall IX64.xmms_modified_stdcall Interop.down_mem c n dom [] _ _ (W.mk_prediction c dom [] (v c IA.win))
+let call_c : call_c_t = IX64.wrap_weak IX64.max_stdcall IX64.arg_reg_stdcall IX64.regs_modified_stdcall IX64.xmms_modified_stdcall Interop.down_mem c n dom (W.mk_prediction c dom [] (v c IA.win))
 let call_c_normal_t : normal call_c_t = as_normal_t #call_c_t call_c
 //You can ask emacs to show you the type of call_c_normal_t ...
 
@@ -90,7 +90,7 @@ let vm_lemma'
        vm_pre code dst src va_s0 sb)
      (ensures (fun (va_s1, f) ->
        V.eval_code code va_s0 f va_s1 /\
-       VSig.vale_calling_conventions va_s0 va_s1 /\
+       VSig.vale_calling_conventions_stdcall va_s0 va_s1 /\
        vm_post code dst src va_s0 sb va_s1 f /\
        ME.buffer_readable VS.(va_s1.mem) (as_vale_immbuffer src) /\
        ME.buffer_readable VS.(va_s1.mem) (as_vale_buffer dst) /\ 
@@ -117,7 +117,7 @@ let vm_lemma'
     va_s1, f
 
 (* Prove that vm_lemma' has the required type *)
-let vm_lemma = as_t #(VSig.vale_sig vm_pre vm_post) vm_lemma'
+let vm_lemma = as_t #(VSig.vale_sig_stdcall vm_pre vm_post) vm_lemma'
 
 let code_memcpy = VM.va_code_memcpy IA.win
 
@@ -244,12 +244,12 @@ let aesni_lemma'
        aesni_pre code va_s0 sb)
      (ensures (fun (va_s1, f) ->
        V.eval_code code va_s0 f va_s1 /\
-       VSig.vale_calling_conventions va_s0 va_s1 /\
+       VSig.vale_calling_conventions_stdcall va_s0 va_s1 /\
        aesni_post code va_s0 sb va_s1 f))
  = VC.va_lemma_check_aesni_stdcall code va_s0 IA.win (as_vale_buffer sb)
 
 (* Prove that vm_lemma' has the required type *)
-let aesni_lemma = as_t #(VSig.vale_sig aesni_pre aesni_post) aesni_lemma'
+let aesni_lemma = as_t #(VSig.vale_sig_stdcall aesni_pre aesni_post) aesni_lemma'
 
 let code_aesni = VC.va_code_check_aesni_stdcall IA.win
 
