vale/specs/interop/Interop.X64.fst
@@ -8,7 +8,7 @@ module TS = X64.Taint_Semantics_s
 module IA = Interop.Assumptions
 module ST = FStar.HyperStack.ST
 
-let wrap_variadic c n arg_reg down_mem num_b8_slots args #pre_rel #post_rel predict =
+let wrap_variadic c n arg_reg regs_modified xmms_modified down_mem num_b8_slots args #pre_rel #post_rel predict =
   let h0 = ST.get () in
   let h0' = h0 in
   assert (mem_roots_p h0' args);
@@ -47,6 +47,8 @@ let wrap_variadic c n arg_reg down_mem num_b8_slots args #pre_rel #post_rel pred
 let rec wrap_aux
     (n:nat)
     (arg_reg:arg_reg_relation n)
+    (regs_modified:MS.reg -> bool)
+    (xmms_modified:MS.xmm -> bool)    
     (down_mem:down_mem_t)
     (c:TS.tainted_code)
     (num_b8_slots:max_slots)
@@ -54,8 +56,8 @@ let rec wrap_aux
     (args:list arg{arity_ok_2 n dom args})
     (pre_rel:rel_gen_t n c dom args (prediction_pre_rel_t n c))
     (post_rel:rel_gen_t n c dom args (prediction_post_rel_t n c num_b8_slots))
-    (predict:prediction_t n arg_reg down_mem c num_b8_slots dom args pre_rel post_rel)
-  : as_lowstar_sig_t n arg_reg down_mem c num_b8_slots dom args pre_rel post_rel predict
+    (predict:prediction_t n arg_reg regs_modified xmms_modified down_mem c num_b8_slots dom args pre_rel post_rel)
+  : as_lowstar_sig_t n arg_reg regs_modified xmms_modified down_mem c num_b8_slots dom args pre_rel post_rel predict
   = match dom with
     | [] ->
       let f () :
@@ -63,25 +65,27 @@ let rec wrap_aux
            (requires fun h0 ->
              mem_roots_p h0 args /\ elim_rel_gen_t_nil pre_rel h0)
            (ensures fun h0 ret h1 ->
-             as_lowstar_sig_post n arg_reg down_mem c num_b8_slots args h0 #pre_rel #post_rel (elim_predict_t_nil predict) ret h1) =
-        wrap_variadic c n arg_reg down_mem num_b8_slots args (elim_predict_t_nil predict)
+             as_lowstar_sig_post n arg_reg regs_modified xmms_modified down_mem c num_b8_slots args h0 #pre_rel #post_rel (elim_predict_t_nil predict) ret h1) =
+        wrap_variadic c n arg_reg regs_modified xmms_modified down_mem num_b8_slots args (elim_predict_t_nil predict)
       in
-      f <: as_lowstar_sig_t n arg_reg down_mem c num_b8_slots [] args pre_rel post_rel predict
+      f <: as_lowstar_sig_t n arg_reg regs_modified xmms_modified down_mem c num_b8_slots [] args pre_rel post_rel predict
 
     | hd::tl ->
       fun (x:td_as_type hd) ->
-      wrap_aux n arg_reg down_mem c num_b8_slots tl
+      wrap_aux n arg_reg regs_modified xmms_modified down_mem c num_b8_slots tl
         (x ++ args)
         (elim_rel_gen_t_cons hd tl pre_rel x)
         (elim_rel_gen_t_cons hd tl post_rel x)
         (elim_predict_t_cons hd tl predict x)
 
-let wrap n arg_reg down_mem c num_b8_slots dom #pre_rel #post_rel predict =
-  wrap_aux n arg_reg down_mem c num_b8_slots dom [] pre_rel post_rel predict
+let wrap n arg_reg regs_modified xmms_modified down_mem c num_b8_slots dom #pre_rel #post_rel predict =
+  wrap_aux n arg_reg regs_modified xmms_modified down_mem c num_b8_slots dom [] pre_rel post_rel predict
 
 let rec wrap_aux_weak
     (n:nat)
     (arg_reg:arg_reg_relation n)
+    (regs_modified:MS.reg -> bool)
+    (xmms_modified:MS.xmm -> bool)
     (down_mem:down_mem_t)
     (c:TS.tainted_code)
     (num_b8_slots:max_slots)
@@ -89,8 +93,8 @@ let rec wrap_aux_weak
     (args:list arg{arity_ok_2 n dom args})
     (pre_rel:rel_gen_t n c dom args (prediction_pre_rel_t n c))
     (post_rel:rel_gen_t n c dom args (prediction_post_rel_t n c num_b8_slots))
-    (predict:prediction_t n arg_reg down_mem c num_b8_slots dom args pre_rel post_rel)
-  : as_lowstar_sig_t_weak n arg_reg down_mem c num_b8_slots dom args pre_rel post_rel predict
+    (predict:prediction_t n arg_reg regs_modified xmms_modified down_mem c num_b8_slots dom args pre_rel post_rel)
+  : as_lowstar_sig_t_weak n arg_reg regs_modified xmms_modified down_mem c num_b8_slots dom args pre_rel post_rel predict
   = match dom with
     | [] ->
       let f () 
@@ -99,20 +103,20 @@ let rec wrap_aux_weak
              mem_roots_p h0 args /\ elim_rel_gen_t_nil pre_rel h0)
            (ensures fun h0 ret h1 ->
              as_lowstar_sig_post_weak
-               n arg_reg
+               n arg_reg regs_modified xmms_modified
                down_mem c num_b8_slots args h0 
                #pre_rel #post_rel (elim_predict_t_nil predict) ret h1)
-        = wrap_variadic c n arg_reg down_mem num_b8_slots args (elim_predict_t_nil predict)
+        = wrap_variadic c n arg_reg regs_modified xmms_modified down_mem num_b8_slots args (elim_predict_t_nil predict)
       in
-      f <: as_lowstar_sig_t_weak n arg_reg down_mem c num_b8_slots [] args pre_rel post_rel predict
+      f <: as_lowstar_sig_t_weak n arg_reg regs_modified xmms_modified down_mem c num_b8_slots [] args pre_rel post_rel predict
 
     | hd::tl ->
       fun (x:td_as_type hd) ->
-      wrap_aux_weak n arg_reg down_mem c num_b8_slots tl
+      wrap_aux_weak n arg_reg regs_modified xmms_modified down_mem c num_b8_slots tl
         (x ++ args)
         (elim_rel_gen_t_cons hd tl pre_rel x)
         (elim_rel_gen_t_cons hd tl post_rel x)
         (elim_predict_t_cons hd tl predict x)
 
-let wrap_weak n arg_reg down_mem c num_b8_slots dom #pre_rel #post_rel predict =
-  wrap_aux_weak n arg_reg down_mem c num_b8_slots dom [] pre_rel post_rel predict
+let wrap_weak n arg_reg regs_modified xmms_modified down_mem c num_b8_slots dom #pre_rel #post_rel predict =
+  wrap_aux_weak n arg_reg regs_modified xmms_modified down_mem c num_b8_slots dom [] pre_rel post_rel predict
